disallowed break/continue where it shouldn't be

L10/Interpret.v
@@ -68,6 +68,8 @@ Fixpoint interpret_call {call_depth_bound: nat}
               in (world', match result with
                           | StmtSuccess => ExprSuccess zero256
                           | StmtReturnFromFunction x => ExprSuccess x
+                          | StmtAbort AbortBreak
+                          | StmtAbort AbortContinue => expr_error "break and continue not allowed"
                           | StmtAbort a => ExprAbort a
                           end)
           end
