L40Metered/Call.v
@@ -1,0 +1,190 @@
+From Coq Require Import String Arith ZArith PropExtensionality Lia.
+
+From Vyper Require Import Config Calldag.
+From Vyper.L10 Require Import Base.
+From Vyper.L40 Require Import AST Descend Callset Descend Expr Stmt Interpret.
+From Vyper.L40Metered Require Import Interpret Expr Stmt.
+
+Lemma call_metering_ok
+           {C: VyperConfig}
+           {bigger_call_depth_bound smaller_call_depth_bound: nat}
+           (Ebound: bigger_call_depth_bound = S smaller_call_depth_bound)
+           {max_call_depth: nat}
+           (DepthOk: bigger_call_depth_bound <= max_call_depth)
+           {cd: calldag}
+           (fc: fun_ctx cd bigger_call_depth_bound)
+           (builtins: string -> option builtin)
+           (world: world_state)
+           (arg_values: list uint256):
+  let '(world', result) := interpret_call builtins fc world arg_values
+   in interpret_call_metered max_call_depth (cd_decls cd) builtins (fun_decl fc)
+                             world arg_values
+       =
+      (world', Some result).
+Proof.
+revert smaller_call_depth_bound Ebound fc world arg_values max_call_depth DepthOk.
+induction bigger_call_depth_bound; intros. { discriminate. }
+inversion Ebound. subst. clear Ebound.
+unfold interpret_call. fold (@interpret_call C smaller_call_depth_bound cd).
+match goal with
+|- let '(world', result) :=
+     match fun_decl fc as d with
+     | FunDecl name arity body => ?X
+     end eq_refl
+   in _ = _
+    =>
+   remember (fun name arity body => X) as do_call
+end.
+enough (Q: forall name arity body E,
+           let '(world', result) := do_call name arity body E in
+           interpret_call_metered max_call_depth (cd_decls cd) builtins
+                                  (FunDecl name arity body) world arg_values
+            =
+           (world', Some result)).
+{
+  clear Heqdo_call.
+  destruct (fun_decl fc) as (name, arity, body).
+  apply Q.
+}
+intros. subst do_call.
+unfold interpret_call_metered.
+destruct max_call_depth. { apply Nat.nle_succ_0 in DepthOk. contradiction. }
+simpl. (* cbn does something weird *)
+fold interpret_call_metered.
+remember (Datatypes.length arg_values =? N.to_nat arity) as arity_ok.
+destruct arity_ok. 2:reflexivity.
+assert (IH: forall (fc': fun_ctx cd smaller_call_depth_bound)
+                   (world: world_state)
+                   (arg_values: list uint256),
+             let
+             '(world', result) := interpret_call builtins fc' world arg_values in
+              interpret_call_metered max_call_depth (cd_decls cd) builtins (fun_decl fc') world arg_values = (world', Some result)).
+{
+  intros.
+  assert (D := fun_bound_ok fc'). rewrite Nat.ltb_lt in D.
+  destruct smaller_call_depth_bound. { apply Nat.nlt_0_r in D. contradiction. }
+  apply (IHbigger_call_depth_bound _ eq_refl).
+  apply (le_S_n _ _ DepthOk).
+}
+assert (M := let _ := memory_impl in
+             block_metering_ok eq_refl fc
+                               (interpret_call builtins)
+                               (interpret_call_metered max_call_depth
+                                                       (cd_decls cd) builtins)
+                               IH builtins world (OpenArray.from_list arg_values) nil
+                               body ((Interpret.interpret_call_helper E))).
+destruct interpret_block as ((world', loc'), result). rewrite M.
+destruct result; try easy.
+now destruct a.
+Qed.
+
+(* XXX this is a dup from somewhere else *)
+Lemma match_some {T R} {x: option T} {y: T} (E: x = Some y)
+                 (some_branch: forall z: T, x = Some z -> R)
+                 (none_branch: x = None -> R):
+  match x as x' return x = x' -> _ with
+  | Some z => some_branch z
+  | None => none_branch
+  end eq_refl
+   =
+  some_branch y E.
+Proof.
+destruct x. 2:discriminate.
+inversion E. subst. f_equal. apply proof_irrelevance.
+Qed.
+
+Lemma match_none {T R} {x: option T} (E: x = None)
+                 (some_branch: forall z: T, x = Some z -> R)
+                 (none_branch: x = None -> R):
+  match x as x' return x = x' -> _ with
+  | Some z => some_branch z
+  | None => none_branch
+  end eq_refl
+   =
+  none_branch E.
+Proof.
+destruct x. 1:discriminate.
+inversion E. subst. f_equal. apply proof_irrelevance.
+Qed.
+
+Fixpoint max_depth_by_names (m: string -> option nat) (l: list string)
+{struct l}
+: nat
+:= match l with
+   | nil => 0
+   | (h :: t)%list => match m h with
+                      | Some n => max n (max_depth_by_names m t)
+                      | None   =>        max_depth_by_names m t
+                      end
+   end.
+
+Definition max_depth_in_calldag {C: VyperConfig}
+                                (cd: calldag)
+:= let _ := string_map_impl in
+   max_depth_by_names (cd_depthmap cd)
+                      (List.map fst (Map.items (cd_decls cd))).
+
+Lemma max_depth_in_calldag_ok {C: VyperConfig}
+                              {cd: calldag}
+                              {name: string}
+                              {d: decl}
+                              {depth: nat}
+                              (Ok: cd_declmap cd name = Some d)
+                              (D: cd_depthmap cd name = Some depth):
+  depth <= max_depth_in_calldag cd.
+Proof.
+unfold cd_declmap in Ok.
+rewrite Map.items_ok in Ok.
+unfold max_depth_in_calldag.
+remember (Map.items (cd_decls cd)) as l. clear Heql.
+induction l as [|(k,v)]. { easy. }
+cbn in *.
+destruct string_dec as [E|NE].
+{ subst k. rewrite D. lia. }
+assert (IH := IHl Ok).
+destruct (cd_depthmap cd k); lia.
+Qed.
+
+Lemma metering_ok
+           {C: VyperConfig}
+           {max_call_depth: nat}
+           {cd: calldag}
+           (DepthOk: max_depth_in_calldag cd < max_call_depth)
+           (builtins: string -> option builtin)
+           (fun_name: string)
+           (world: world_state)
+           (args: list uint256):
+  let '(world', result) := interpret builtins cd fun_name world args
+   in interpret_metered max_call_depth (cd_decls cd) builtins fun_name world args
+       =
+      (world', Some result).
+Proof.
+unfold interpret.
+unfold interpret_metered.
+unfold make_fun_ctx_and_bound.
+unfold cd_declmap. unfold Base.map_lookup.
+refine (match Map.lookup (cd_decls cd) fun_name as z return _ = z -> _ with
+        | Some d => fun E => _
+        | None => fun E => _
+        end eq_refl).
+2:{ rewrite (match_none E). rewrite E. trivial. }
+rewrite (match_some E).
+refine (match cd_depthmap cd fun_name as z return _ = z -> _ with
+        | Some depth => fun D => _
+        | None => fun D => _
+        end eq_refl).
+2:{ exfalso. exact (Calldag.make_fun_ctx_helper E D). }
+rewrite (match_some D).
+assert (M' := max_depth_in_calldag_ok E D).
+assert (M: S depth <= max_call_depth) by lia.
+assert (CM := call_metering_ok eq_refl M {|
+             fun_name := fun_name;
+             fun_depth := depth;
+             fun_depth_ok := D;
+             fun_decl := d;
+             fun_decl_ok := E;
+             fun_bound_ok := proj2 (Nat.ltb_lt depth (S depth)) (Nat.lt_succ_diag_r depth)
+           |} builtins world args).
+destruct interpret_call as (world', result).
+rewrite E. apply CM.
+Qed.
